theory/Abstract_Communication_Soundness.thy
@@ -6,150 +6,6 @@ theory Abstract_Communication_Soundness
     Communication_Analysis Abstract_Communication_Analysis
 begin
 
-lemma path_not_reachable_sound: "
-  \<lbrakk>
-    (\<V>, \<C>) \<Turnstile>\<^sub>e e;
-    [[] \<mapsto> \<langle>e;Map.empty;[]\<rangle>] \<rightarrow>* \<E>';
-    \<E>' \<pi> = Some (\<langle>LET x = b in e';\<rho>';\<kappa>'\<rangle>) 
-  \<rbrakk> \<Longrightarrow>
-  (\<V>, e) :\<downharpoonright> (\<pi>;;`x)
-"
-sorry
-
-lemma nonempty_pool: "
-  \<lbrakk>
-    \<E> \<rightarrow> \<E>'
-  \<rbrakk>\<Longrightarrow>
-  (\<exists> \<pi> e \<rho> \<kappa> \<pi>' e' \<rho>' \<kappa>'. 
-    \<E> \<pi> = Some (\<langle>e;\<rho>;\<kappa>\<rangle>) \<and> 
-    leaf \<E> \<pi> \<and>
-    \<E>' \<pi>' = Some (\<langle>e';\<rho>';\<kappa>'\<rangle>) \<and>
-    prefix \<pi> \<pi>'
-  )
-"
- apply (erule concur_step.cases, auto, blast)
-done
-
-lemma trace_preservation: "
-  \<E> \<rightarrow> \<E>' \<Longrightarrow> 
-  \<E> \<pi> = Some (\<langle>e;\<rho>;\<kappa>\<rangle>) \<Longrightarrow>
-  \<E>' \<pi> = Some (\<langle>e;\<rho>;\<kappa>\<rangle>)
-"
- apply (erule concur_step.cases; (erule seq_step.cases)?; auto)
- apply (metis leaf_def option.distinct(1) strict_prefixI')+
-done
-
-(*
-lemma nonempty_pool_star_left: "
-  \<lbrakk>
-   star_left op \<rightarrow> \<E> \<E>\<^sub>m
-  \<rbrakk>\<Longrightarrow>
-  (\<forall> \<E>'' . \<E>\<^sub>m \<rightarrow> \<E>'' \<longrightarrow> 
-    (*(\<forall> \<pi>'' e'' \<rho>'' \<kappa>''. \<E>'' \<pi>'' = Some (\<langle>e'';\<rho>'';\<kappa>''\<rangle>) \<longrightarrow>*)
-      (\<exists> \<pi> e \<rho> \<kappa> \<pi>\<^sub>m e\<^sub>m \<rho>\<^sub>m \<kappa>\<^sub>m . 
-        \<E> \<pi> = Some (\<langle>e;\<rho>;\<kappa>\<rangle>) \<and> 
-        leaf \<E> \<pi> \<and>
-        \<E>\<^sub>m \<pi>\<^sub>m = Some (\<langle>e\<^sub>m;\<rho>\<^sub>m;\<kappa>\<^sub>m\<rangle>) \<and>
-        prefix \<pi> \<pi>\<^sub>m (*\<and>
-        leaf \<E>\<^sub>m \<pi>\<^sub>m \<and>
-        prefix \<pi>\<^sub>m \<pi>'' *)
-      )
-    (*)*)
-  )
-"
- apply (erule star_left.induct; simp)
-  using nonempty_pool apply blast
- apply (rename_tac \<E> \<E>\<^sub>m \<E>', auto)
- apply ((rule exI)+, (rule conjI)+, (rule exI)+, assumption)
- apply (rule conjI, assumption)
- apply (drule trace_preservation, assumption)
- apply ((rule exI)+, (rule conjI)+, (rule exI)+, assumption)
-sorry
-*)
-
-lemma nonempty_pool_star_left: "
-  \<lbrakk>
-   star_left op \<rightarrow> \<E> \<E>\<^sub>m
-  \<rbrakk>\<Longrightarrow>
-  (\<forall> \<E>'' . \<E>\<^sub>m \<rightarrow> \<E>'' \<longrightarrow> 
-  (\<forall> \<pi> e \<rho> \<kappa>. \<E> \<pi> = Some (\<langle>e;\<rho>;\<kappa>\<rangle>) \<longrightarrow>
-  (\<forall> \<pi>'' e'' \<rho>'' \<kappa>''. \<E>'' \<pi>'' = Some (\<langle>e'';\<rho>'';\<kappa>''\<rangle>) \<longrightarrow>
-      (\<exists> \<pi>\<^sub>m e\<^sub>m \<rho>\<^sub>m \<kappa>\<^sub>m . 
-        \<E> \<pi> = Some (\<langle>e;\<rho>;\<kappa>\<rangle>) \<and> 
-        leaf \<E> \<pi> \<and>
-        \<E>\<^sub>m \<pi>\<^sub>m = Some (\<langle>e\<^sub>m;\<rho>\<^sub>m;\<kappa>\<^sub>m\<rangle>) \<and>
-        prefix \<pi> \<pi>\<^sub>m \<and>
-        leaf \<E>\<^sub>m \<pi>\<^sub>m \<and>
-        prefix \<pi>\<^sub>m \<pi>''
-      )
-   )))
-"
-sorry
-
-lemma exp_not_reachable_sound'': "
-   star_left op \<rightarrow> \<E> \<E>\<^sub>m \<Longrightarrow>
-   \<E>\<^sub>m \<rightarrow> \<E>' \<Longrightarrow>
-   (\<V>, \<C>) \<Turnstile>\<^sub>\<E> \<E> \<Longrightarrow>
-
-   \<forall>\<pi> e. (\<exists>\<rho> \<kappa>. \<E> \<pi> = Some (\<langle>e;\<rho>;\<kappa>\<rangle>)) \<longrightarrow>
-          leaf \<E> \<pi> \<longrightarrow> (\<forall>\<pi>' e'. (\<exists>\<rho>' \<kappa>'. \<E>\<^sub>m \<pi>' = Some (\<langle>e';\<rho>';\<kappa>'\<rangle>)) \<longrightarrow> prefix \<pi> \<pi>' \<longrightarrow> (\<V>, e) \<downharpoonright> e') \<Longrightarrow>
-
-   \<E> \<pi> = Some (\<langle>e;\<rho>;\<kappa>\<rangle>) \<Longrightarrow> leaf \<E> \<pi> \<Longrightarrow> \<E>' \<pi>' = Some (\<langle>e';\<rho>';\<kappa>'\<rangle>) \<Longrightarrow> prefix \<pi> \<pi>' \<Longrightarrow> 
-   (\<V>, e) \<downharpoonright> e'
-"
- apply (frule nonempty_pool_star_left)
- apply (drule star_left_implies_star)
- apply (drule flow_preservation_star, auto)
- apply (drule spec[of _ \<pi>])
- apply (drule spec[of _ \<E>'])
- apply (drule spec[of _ e])
- apply simp
- apply (drule spec[of _ \<pi>])
- apply (erule impE, (rule exI)+, assumption)
- apply (rotate_tac 8)
- apply (drule spec[of _ \<pi>'])
- apply (erule impE, (rule exI)+, assumption)
- apply ((erule conjE), (erule exE), (erule conjE)+, (erule exE)+)
- apply ((drule spec)+, erule impE, (rule exI)+, assumption)
- apply (erule impE, assumption)
- apply (erule accept_state_pool.cases, auto)
- apply ((drule spec)+, erule impE, assumption)
- apply (erule accept_state.cases, auto)
- apply (rename_tac \<pi>\<^sub>m e\<^sub>m \<rho>\<^sub>m \<kappa>\<^sub>m)
- apply (erule concur_step.cases; (erule seq_step.cases)?; auto)
-sorry
-
-lemma exp_not_reachable_sound': "
-  \<lbrakk>
-    \<E> \<rightarrow>* \<E>'
-  \<rbrakk> \<Longrightarrow>
-  (\<V>, \<C>) \<Turnstile>\<^sub>\<E> \<E> \<longrightarrow>
-  (\<forall> \<pi> e \<rho> \<kappa> \<pi>' e' \<rho>' \<kappa>' .
-    \<E> \<pi> = Some (\<langle>e;\<rho>;\<kappa>\<rangle>) \<longrightarrow>
-    leaf \<E> \<pi> \<longrightarrow>
-    \<E>' \<pi>' = Some (\<langle>e';\<rho>';\<kappa>'\<rangle>) \<longrightarrow>
-    prefix \<pi> \<pi>' \<longrightarrow>
-    (\<V>, e) \<downharpoonright> e'
-  )
-"
- apply (drule star_implies_star_left)
- apply (erule star_left.induct, auto)
- apply (metis exp_reachable.Refl leaf_def option.inject option.simps(3) prefix_order.le_imp_less_or_eq state.inject)
- apply (rename_tac \<E> \<E>\<^sub>m \<E>' \<pi> e \<rho> \<kappa> \<pi>' e' \<rho>' \<kappa>')
- apply (insert exp_not_reachable_sound'', auto)
-done
-
-lemma exp_not_reachable_sound: "
-  \<lbrakk>
-    (\<V>, \<C>) \<Turnstile>\<^sub>e e;
-    [[] \<mapsto> \<langle>e;Map.empty;[]\<rangle>] \<rightarrow>* \<E>';
-    \<E>' \<pi>' = Some (\<langle>e';\<rho>';\<kappa>'\<rangle>) 
-  \<rbrakk> \<Longrightarrow>
-  (\<V>, e) \<downharpoonright> e'
-"
- apply (insert exp_not_reachable_sound', auto)
- apply (smt Nil_prefix fun_upd_apply fun_upd_same leaf_def lift_flow_exp_to_pool option.distinct(1) strict_prefix_def)
-done
 
 lemma abstract_chan_doesnt_exist_sound: "
   \<lbrakk>
@@ -240,7 +96,7 @@ lemma isnt_send_path_sound': "
   {^\<lparr>\<rparr>} \<subseteq> \<V> x\<^sub>y \<and> \<V> x\<^sub>m \<subseteq> \<C> x\<^sub>c
 
 "
- apply (rule conjI, (erule path_not_reachable_sound; assumption))
+ apply (rule conjI, (erule path_not_traceable_sound; assumption))
  apply (rule conjI, (erule exp_not_reachable_sound; assumption))
  apply (rule conjI, (erule abstract_chan_doesnt_exist_sound; assumption))
  apply (rule conjI, (erule abstract_send_evt_doesnt_exist_sound; assumption))
@@ -557,7 +413,7 @@ theorem is_abstract_topo_sound: "
     \<A> \<bind> e;
     [[] \<mapsto> \<langle>e; empty; []\<rangle>] \<rightarrow>* \<E>'
   \<rbrakk> \<Longrightarrow>
-  \<langle>\<langle>\<E>'; \<pi>\<rangle>\<rangle> \<sqsubseteq>\<^sub>t \<A>
+  \<langle>\<langle>\<E>'; \<pi>\<rangle>\<rangle> \<sqsubseteq>\<^sub>t \<A> 
 "
  apply (unfold topo_accept_def)
  apply (unfold topo_env_precision_def)
